Get all possible conv enter sequences

LeanAide/GoalLocations.lean
@@ -4,193 +4,57 @@ import Std
 
 open Lean Meta Expr 
 
-def Lean.Expr.getConvEnters : Expr → MetaM (Array (List String × Expr))
-  | .app _ _ => _
-  | .forallE _ _ _ _ => _
-  | .lam _ _ _ _ 
-  | .letE _ _ _ _ _ => _
-  | .mdata _ expr => _
-  | .proj _ _ struct => _
-  | _ => _
+-- TODO Check whether this function already exists
+def Lean.Expr.getName! : Expr → Name
+  | .lam n _ _ _ => n
+  | .letE n _ _ _ _ => n
+  | .forallE n _ _ _ => n
+  | _               => panic! "Unable to get name for expression."
 
-
-def Lean.SubExpr.extensions (p : SubExpr.Pos) : Expr → MetaM (Array (SubExpr.Pos × Expr))
-  | .app fn arg => do
-    let fnf ← whnf fn
-    if fnf.binderInfoEx == .default then
-      if fnf.isApp then
-        return #[(p.pushAppFn, fnf), (p.pushAppArg, arg)]
-      else
-        return #[(p.pushAppArg, arg)]
-    else return #[]
-  | .lam _ _ body _ => return #[(p.pushBindingBody, body)]
-  | .forallE _ _ body _ => return #[(p.pushBindingBody, body)]
-  | .letE _ type value body _ => 
-    return #[(p.pushLetVarType, type), (p.pushLetValue, value), (p.pushLetBody, body)]
-  | .mdata _ expr => extensions p expr
-  | .proj _ _ struct => return #[(p.pushProj, struct)]
-  |  _ => return #[]
-
-partial def Lean.Expr.allSubExprs (p : SubExpr.Pos) (e : Expr) : MetaM (Array (SubExpr.Pos × Expr)) := do
-  let exts ← Lean.SubExpr.extensions p e
-  let rexts ← exts.concatMapM fun (pos, subexpr) ↦ allSubExprs pos subexpr 
-  return rexts.push (p, e)
-
-def Lean.Expr.allPositions (e : Expr) : MetaM (Array SubExpr.Pos) := do
-  let exprs ← e.allSubExprs .root
-  return exprs.map Prod.fst
-
-def Lean.Expr.viewPositions (e : Expr) : MetaM (Array (SubExpr.Pos × String)) := do
-  let exprs ← e.allSubExprs .root
-  exprs.mapM fun (pos, subexpr) ↦ do
-    let stx ← PrettyPrinter.delab subexpr
-    return (pos, stx.raw.reprint.get!)
-
-open Meta Elab Term in
-#eval show TermElabM _ from do
-  let stx ← `(term| 1 + 2) 
-  let t ← Term.elabTerm stx none
-  let t ← reduce t
-  return t.allPositions
-
--- The code below has been modified from `ProofWidgets/Demos/Conv`,
--- copyright of Robin Böhne and Wojciech Nawrocki.
-
-private structure SolveReturn where
-  expr : Expr
-  val? : Option String
-  listRest : List Nat
-
-private def solveLevel (expr : Expr) (path : List Nat) : MetaM SolveReturn := match expr with
-  | .app _ _ => do
-    let mut descExp := expr
-    let mut count := 0
-    let mut explicitList := []
-
-    -- we go through the application until we reach the end, counting how many explicit arguments it has and noting whether
-    -- they are explicit or implicit
-    while descExp.isApp do
-      if (←Lean.Meta.inferType descExp.appFn!).bindingInfo!.isExplicit then
-        explicitList := true::explicitList
-        count := count + 1
-      else
-        explicitList := false::explicitList
-      descExp := descExp.appFn!
-
-    -- we get the correct `enter` command by subtracting the number of `true`s in our list
-    let mut mutablePath := path
-    let mut length := count
-    explicitList := List.reverse explicitList
-    while !mutablePath.isEmpty && mutablePath.head! == 0 do
-      if explicitList.head! == true then
-        count := count - 1
-      explicitList := explicitList.tail!
-      mutablePath := mutablePath.tail!
-
-    let mut nextExp := expr
-    while length > count do
-      nextExp := nextExp.appFn!
-      length := length - 1
-    nextExp := nextExp.appArg!
-
-    let pathRest := if mutablePath.isEmpty then [] else mutablePath.tail!
-
-    return { expr := nextExp, val? := toString count , listRest := pathRest }
-
-  | .lam n _ b _ => pure { expr := b, val? := n.getString!, listRest := path.tail! }
-  | .forallE n _ b _ => pure { expr := b, val? := n.getString!, listRest := path.tail! }
-
-  | .mdata _ b => do
-    match b with
-      | Expr.mdata _ _ => return { expr := b, val? := none, listRest := path }
-      | _ => return { expr := b.appFn!.appArg!, val? := none, listRest := path.tail!.tail! }
-
-  | _ => do
-    return { expr := ←(Lean.Core.viewSubexpr path.head! expr), val? := toString (path.head! + 1), listRest := path.tail! }
-
-private def solveLevel' (expr : Expr) (path : List Nat) : MetaM SolveReturn := match expr with
+partial def Lean.Expr.getConvEnters (expr : Expr) (explicit? : Bool) : MetaM (Array (List String × Expr)) :=
+  match expr with
   | .app _ _ => do
     let fn := expr.getAppFn 
     let args := expr.getAppArgs
     let fnInfo ← getFunInfo fn
-    let explicitArr := fnInfo.paramInfo.map (·.isExplicit) 
-    let mut descExp := expr
-    let mut count := 0
-    let mut explicitList := []
+    let argsWithBinderInfo := Array.zip args (fnInfo.paramInfo.map (·.isExplicit))
+    let args' :=
+      argsWithBinderInfo.filterMap <| fun (arg, bi) ↦
+        if explicit? || (!explicit? && bi) then
+          some arg
+        else none
+    let enterArgs ← args'.mapIdxM fun idx arg ↦ do
+      let argConvEnters ← arg.getConvEnters explicit?
+      let enterArg := (if explicit? then "@" else "") ++ s!"{idx.val + 1}"
+      return argConvEnters.map <| fun (path, subexpr) ↦
+        (enterArg :: path, subexpr)
+    (enterArgs.push #[([], expr)]).concatMapM pure  
+  | .forallE _ _ _ _ => do
+    let binders := expr.getForallBinderNames |>.map Name.toString
+    let body := expr.getForallBody
+    let bodyConvEnters ← body.getConvEnters explicit?
+    return (bodyConvEnters.map  fun (path, subexpr) ↦ 
+              (binders ++ path, subexpr)) |>.push ([], expr)  
+  | .lam _ _ _ _ 
+  | .letE _ _ _ _ _ =>
+    lambdaLetTelescope expr <| fun args body ↦ do
+      let binders := args |>.map (·.getName!.toString) |>.toList
+      let bodyConvEnters ← body.getConvEnters explicit?
+      return (bodyConvEnters.map  fun (path, subexpr) ↦
+                (binders ++ path, subexpr)) |>.push ([], expr)
+  | .mdata _ expr => getConvEnters expr explicit?
+  | .proj _ _ struct => do
+    let structConvEnters ← struct.getConvEnters explicit?
+    return (structConvEnters.map fun (path, subexpr) ↦
+                  ("1" :: path, subexpr)) |>.push ([], expr)
+  | _ => return #[([], expr)]
 
-    -- we go through the application until we reach the end, counting how many explicit arguments it has and noting whether
-    -- they are explicit or implicit
-    while descExp.isApp do
-      if (←Lean.Meta.inferType descExp.appFn!).bindingInfo!.isExplicit then
-        explicitList := true::explicitList
-        count := count + 1
-      else
-        explicitList := false::explicitList
-      descExp := descExp.appFn!
-
-    -- we get the correct `enter` command by subtracting the number of `true`s in our list
-    let mut mutablePath := path
-    let mut length := count
-    explicitList := List.reverse explicitList
-    while !mutablePath.isEmpty && mutablePath.head! == 0 do
-      if explicitList.head! == true then
-        count := count - 1
-      explicitList := explicitList.tail!
-      mutablePath := mutablePath.tail!
-
-    let mut nextExp := expr
-    while length > count do
-      nextExp := nextExp.appFn!
-      length := length - 1
-    nextExp := nextExp.appArg!
-
-    let pathRest := if mutablePath.isEmpty then [] else mutablePath.tail!
-
-    return { expr := nextExp, val? := toString count , listRest := pathRest }
-
-  | .lam n _ b _ => pure { expr := b, val? := n.getString!, listRest := path.tail! }
-  | .forallE n _ b _ => pure { expr := b, val? := n.getString!, listRest := path.tail! }
-
-  | .mdata _ b => do
-    match b with
-      | Expr.mdata _ _ => return { expr := b, val? := none, listRest := path }
-      | _ => return { expr := b.appFn!.appArg!, val? := none, listRest := path.tail!.tail! }
-
-  | _ => do
-    return { expr := ←(Lean.Core.viewSubexpr path.head! expr), val? := toString (path.head! + 1), listRest := path.tail! }
-
-def Lean.SubExpr.Pos.toConvEnterArg (goalType : Expr) (subexprPos : SubExpr.Pos) : MetaM (List String) := do
-  let mut list := subexprPos.toArray.toList
-  let mut expr := goalType
-  let mut retList := []
-  -- generate list of commands for `enter`
-  while !list.isEmpty do
-    let res ← solveLevel expr list
-    expr := res.expr
-    retList := match res.val? with
-      | none => retList
-      | some val => val::retList
-    list := res.listRest
-
-  -- build `enter [...]` string
-  retList := List.reverse retList
-  return retList
-
-def Lean.Expr.allConvEnterArgs (e : Expr) : MetaM <| Array (List String) := do
-  (← e.allPositions).filterMapM <| fun pos ↦
-    try? do Lean.SubExpr.Pos.toConvEnterArg e pos
-
-open Elab Term
-
-def testExpr := do
+open Meta Elab Term in
+#eval show TermElabM _ from do
   let stx ← `(term| ∀ x, Nat.succ x = 1) 
-  Term.elabTerm stx none
-
--- #eval (SubExpr.Pos.fromString! "/1").toConvEnterArg <$> testExpr
-
-#check FunInfo
-#check getFunInfo
-#check getAppArgs'
-
-example : ∀ x : 1 + 2 = 3, x = x := by
-  conv 
+  let t ← Term.elabTerm stx none
+  let enters ← t.getConvEnters (explicit? := false)
+  for (path, expr) in enters do
+    IO.println path
+    let stx ← PrettyPrinter.delab expr
+    IO.println stx.raw.reprint.get!
